Refactor definition of vale_heap_layout_inner

vale/code/arch/Vale.Arch.HeapImpl.fst
@@ -4,6 +4,9 @@ open Vale.Interop
 open Vale.Def.Words_s
 open Vale.Arch.MachineHeap_s
 open Vale.Interop.Heap_s
+module DV = LowStar.BufferView.Down
+
+let buffer t = (b:b8{DV.length (get_downview b.bsrc) % view_n t == 0})
 
 noeq type vale_heap =
   | ValeHeap:
@@ -16,9 +19,9 @@ noeq type vale_heap_layout_inner : Type u#1 = {
   vl_heaplets_initialized:bool;
   vl_heaplet_map:int -> option heaplet_id; // each address is owned by at most one heaplet
   vl_heaplet_sets:heaplet_id -> Set.set int; // addresses owned by each heaplet (redundant with vl_heaplet_map, but convenient)
-  vl_old_heap:vale_heap; // would go in vl_v, but can't because it is Type u#1
-  vl_t:Type0;
-  vl_v:vl_t; // rest of fields are defined by Vale.X64.Memory
+  vl_old_heap:vale_heap;
+  vl_buffers:Seq.seq buffer_info;
+  vl_mod_loc:LowStar.Modifies.loc;
 }
 
 let empty_vale_heap_layout_inner (h:vale_heap) : vale_heap_layout_inner = {
@@ -26,8 +29,8 @@ let empty_vale_heap_layout_inner (h:vale_heap) : vale_heap_layout_inner = {
   vl_heaplet_map = (fun _ -> None);
   vl_heaplet_sets = (fun _ -> Set.empty);
   vl_old_heap = h;
-  vl_t = unit;
-  vl_v = ();
+  vl_buffers = Seq.empty;
+  vl_mod_loc = LowStar.Modifies.loc_none;
 }
 
 let empty_heaplet (h:vale_heap) (n:nat{n < 16}) : vale_heap =
